proved that sort refines sort_spec up to two lemmas that are solely about lists, not itrees

theories/Merge.v
@@ -4,11 +4,11 @@ Locate "<=?".
 
 Require Import Coq.Lists.List Coq.Sorting.Permutation.
 
-From Coq Require Export Morphisms Setoid Program.Equality.
+From Coq Require Export Morphisms RelationClasses Setoid Program.Equality.
 From ITree Require Export ITree ITreeFacts Eq.Rutt.
 From Paco Require Import paco.
 From Coq Require Export Eqdep EqdepFacts.
-
+Require Import Lia.
 Require Export Refinement.
 
 Import Monads.
@@ -63,9 +63,21 @@ Proof.
 Qed.
 
 (*rec_fix*)
+(* call *)
+Definition call_spec {E A B} (a : A) : itree_spec (callE A B +' E) B :=  
+  ITree.trigger (Spec_vis (inl1 (Call a) ) ).
 
-Definition halve {E} : list nat -> itree E (list nat * list nat) :=
-    rec_fix (fun halve_rec l =>
+Definition rec_spec {E A B} (body : A -> itree_spec (callE A B +' E) B ) (a : A) :
+  itree_spec E B :=
+  mrec_spec (calling' body) (Call a).
+
+Definition rec_fix_spec {E A B} 
+(body : (A -> itree_spec (callE A B +' E) B) -> 
+        A -> itree_spec (callE A B +' E) B  )  :
+  A -> itree_spec E B := rec_spec (body call_spec).
+
+Definition halve {E} : list nat -> itree_spec E (list nat * list nat) :=
+    rec_fix_spec (fun halve_rec l =>
                match l with
                | x :: y :: t => '(l1,l2) <- halve_rec t;; Ret (x :: l1, y :: l2)
                | x :: nil => Ret ( x :: nil  , nil )
@@ -126,6 +138,8 @@ Proof.
   setoid_rewrite bind_ret_l. pstep. constructor. auto. constructor. pstep_reverse.
 Qed.
 
+Opaque assume_spec.
+
 Definition spec_exists {E} (T : Type) : itree_spec E T :=
   trigger (@Spec_exists E T).
 
@@ -171,6 +185,10 @@ Ltac eexistssr := eapply padded_spec_exists_elim.
 
 Ltac existssl := apply padded_spec_exists_eliml.
 
+Ltac assumesr := apply padded_assume_pad_elim.
+Ltac assumesl := apply padded_assume_pad_eliml.
+Ltac assertsr := apply padded_assert_pad_elim.
+Ltac assertsl := apply padded_assert_pad_eliml.
 
 Definition spec_forall {E} (T : Type) : itree_spec E T :=
   trigger (@Spec_forall E T).
@@ -207,14 +225,17 @@ Proof.
   pstep. econstructor. constructor. pstep_reverse.
 Qed.
 
+
+
 Definition halve_spec {E} (l : list nat) : itree_spec E (list nat * list nat) :=
   l1 <- spec_exists (list nat);; 
   l2 <- spec_exists (list nat);;
   assert_spec (Permutation l (l1 ++ l2) );;
+  assert_spec (length l1 >= length l2 /\ (length l > length l1 \/ length l <= 1) );;
   Ret (l1, l2).
 
-Definition merge {E} : (list nat * list nat) -> itree E (list nat) :=
-  rec_fix ( fun merge_rec '(l1, l2) =>
+Definition merge {E} : (list nat * list nat) -> itree_spec E (list nat) :=
+  rec_fix_spec ( fun merge_rec '(l1, l2) =>
               match (l1,l2) with
               | (h1 :: t1, h2 :: t2) => if Nat.leb h1 h2
                                      then
@@ -241,9 +262,17 @@ Definition merge_spec2 {E} l1 l2 : itree_spec E (list nat) :=
 Definition merge_spec {E} l1 l2 : itree_spec E (list nat) := 
   and_spec (merge_spec1 l1 l2) (merge_spec2 l1 l2).
 
+Definition merge_spec' {E} l1 l2 : itree_spec E (list nat) :=
+  assume_spec (sorted l1);;
+  assume_spec (sorted l2);;
+  l <- spec_exists (list nat);;
+  assert_spec (sorted l);;
+  assert_spec (Permutation l (l1 ++ l2));;
+  Ret l.
+
 (*missing base case*)
-Definition sort {E} : list nat -> itree E (list nat) :=
-  rec_fix (fun sort_rec l => 
+Definition sort {E} : list nat -> itree_spec E (list nat) :=
+  rec_fix_spec (fun sort_rec l => 
              if Nat.leb (length l) 1
              then Ret l
              else
@@ -263,6 +292,10 @@ Definition sort_spec {E} (l : list nat) : itree_spec E (list nat) :=
 Definition padded_refines_eq {E R1 R2} RR (phi1 : itree_spec E R1) (phi2 : itree_spec E R2) :=
   padded_refines eqE eqEAns RR phi1 phi2.
 
+Instance proper_leq : Proper (le ==> le ==> le) plus.
+Proof.
+  repeat intro. lia. Qed.
+
 Global Instance padded_refines_eq_refl {E R} : Reflexive (@padded_refines_eq E R R eq).
 Proof.
   red. intros. unfold padded_refines_eq, padded_refines. apply refl_refines; auto.
@@ -271,25 +304,99 @@ Proof.
   - apply pad_is_padded.
 Qed.
 
+Global Instance refines_proper_bind E R S :
+  Proper (@padded_refines_eq E R R eq ==> pointwise_relation _ (padded_refines_eq eq) ==> @padded_refines_eq E S S  eq ) ITree.bind.
+Proof.
+  repeat intro. subst. unfold padded_refines_eq in *. eapply padded_refines_bind; eauto.
+  intros; subst. auto.
+Qed.
+
+Global Instance refines_proper_subst E R S (k : R -> itree_spec E S) : 
+  Proper (@padded_refines_eq E R R eq ==> padded_refines_eq eq) (ITree.subst k).
+Proof.
+  repeat intro. eapply refines_proper_bind. auto. intro. reflexivity.
+Qed.
+
+Global Instance refines_proper_bind_eq E R S :
+  Proper (@padded_refines_eq E R R eq ==> eq ==> @padded_refines_eq E S S  eq ) ITree.bind.
+Proof.
+  repeat intro. eapply refines_proper_bind. auto. subst. intro. reflexivity.
+Qed.
+
+Lemma eqE_eq_type E A B (ea : E A) (eb : E B) : eqE A B ea eb -> A = B.
+Proof.
+  intros. inv H. auto.
+Qed.
+
+Lemma eqE_eq E A (e1 : E A) (e2 : E A) : eqE A A e1 e2 -> e1 = e2.
+Proof.
+  intros. inv H. inj_existT. subst. auto.
+Qed.
+
+Lemma eqEAns_eq_type E A B (ea : E A) (eb : E B) a b : eqEAns A B ea eb a b -> A = B.
+Proof.
+  intros. inv H. auto.
+Qed.
+
+Lemma eqEAns_eq E A (e1 : E A) (e2 : E A) a1 a2 : eqEAns A A e1 e2 a1 a2 -> e1 = e2 /\ a1 = a2.
+Proof.
+  intros. inv H. inj_existT. subst. auto.
+Qed.
+
+Ltac eqE_inv H := apply eqE_eq_type in H as ?H; subst; apply eqE_eq in H; subst.
+Ltac eqEAns_inv H := apply eqEAns_eq_type in H as ?H; subst; apply eqEAns_eq in H as [?H ?H]; subst.
+
 Global Instance padded_refines_eq_trans {E R} : Transitive (@padded_refines_eq E R R eq).
 Proof.
   intros phi1 phi2 phi3 Hphi12 Hphi23. unfold padded_refines_eq, padded_refines in *.
   eapply refines_monot; try eapply refinesTrans; eauto with solve_padded; try apply pad_is_padded.
-  - intros. assert (A = B). inv PR. auto. subst.  assert (ea = eb). inv PR. inj_existT.
-    subst. auto. subst. assert (x0 = x1). inv PR. inj_existT. subst. auto.
-    subst. clear PR. constructor. intros. destruct H. inv H. inj_existT. subst.
-    inv H0. inj_existT. subst. exists x1.
-    split; constructor.
-  - intros. inv PR. inj_existT. subst. 
-    assert (A = B0). inv H3. auto. subst. assert (B = B0). inv H4. auto.
-    subst. assert (x0 = e2). inv H3. inj_existT. subst. auto. subst. auto.
+  - intros A B ea eb PR. assert (A = B). inv PR. inv H3. inv H4. auto. subst.
+    assert (ea = eb). inv PR. inj_existT.
+    subst. assert (B = B0). inv H3. auto. subst. inv H4. inj_existT. subst. inv H3. inj_existT.
+    subst. auto. subst. constructor.
+  - intros.
+    assert (A = B). inv PR. auto. subst. assert (ea = eb). inv PR. inj_existT. subst. auto.
+    subst. constructor. intros. destruct H. assert (x0 = x1). inv PR. inj_existT. subst. auto.
+    subst. assert (B = B0). inv H. auto. subst. exists x1.
+    assert (e2 = eb). inv H. inj_existT. subst. auto. subst. repeat constructor.
   - intros. inv PR. auto.
 Qed.
+
+Global Instance refines_proper_interp_mrec_spec E D R : 
+  Proper ((fun ctx1 ctx2 => forall T d, padded_refines_eq  eq (ctx1 T d) (ctx2 T d) ) ==> @padded_refines_eq (D +' E) R R eq ==> @padded_refines_eq E R R eq) 
+         (fun ctx => @interp_mrec_spec D E ctx R).
+Proof.
+  repeat intro. subst. unfold padded_refines_eq in *.
+  eapply padded_refines_interp_mrec with (REInv := eqE) (REAnsInv := eqEAns) ; eauto.
+  - intros. 
+    eqE_inv H1.
+    eapply refines_monot; try eapply H.
+    + intros.  eqE_inv PR. destruct x2; repeat constructor.
+    + intros. inv PR; inj_existT; subst; eqEAns_inv H7; constructor.
+    + intros. subst. constructor.
+  - eapply refines_monot; try eapply H0.
+    + intros. eqE_inv PR. destruct x2; repeat constructor.
+    + intros. inv PR; inj_existT; subst; eqEAns_inv H7; constructor.
+    + auto.
+Qed.
+
+Global Instance refines_proper_interp_mrec_spec_eq E D R : 
+  Proper (eq ==> @padded_refines_eq (D +' E) R R eq ==> @padded_refines_eq E R R eq) 
+         (fun ctx => @interp_mrec_spec D E ctx R).
+Proof.
+  repeat intro.
+  apply refines_proper_interp_mrec_spec; auto.
+  intros. subst. reflexivity.
+Qed.
+
+
 (*
 Global Instance padded_refines_eq_bind_proper  E1 E2 RE REAns R1 R2 RR : 
   Proper (padded_refines_eq eq ==> eq ==> @padded_refines E1 E2 R1 R2 RE REAns RR ) ITree.bind.
 *)
 (*from there there is a bit more *)
+
+(*need at least bind and ret rules for interp_mrec_spec *)
 
 Lemma interp_mrec_ret : 
   forall {D E : Type -> Type} (ctx : forall T : Type, D T -> itree (D +' E) T) R (r :R),
@@ -313,30 +420,330 @@ Lemma halve_correct E l : padded_refines_eq eq (halve l) (@halve_spec E l).
 Proof.
   revert l.
   apply list_ind2_principle.
-  - unfold halve, halve_spec, rec_fix, rec, mrec. cbn.
-    rewrite interp_mrec_ret. existssr (@nil nat). existssr (@nil nat). 
-    apply padded_assert_pad_elim. constructor. 
+  - unfold halve, halve_spec, rec_fix_spec, rec_spec, mrec_spec. cbn.
+    rewrite interp_mrec_spec_ret. existssr (@nil nat). existssr (@nil nat). 
+    assertsr. reflexivity. assertsr. split; auto.
     reflexivity.
-  - intros n. cbn. unfold halve, halve_spec, rec_fix, rec, mrec. cbn.
-    rewrite interp_mrec_ret. existssr ( n :: nil ). existssr (@nil nat).
-    apply padded_assert_pad_elim. cbn. repeat constructor.
+  - intros n. unfold halve, halve_spec, rec_fix_spec, rec_spec, mrec_spec. cbn.
+    rewrite interp_mrec_spec_ret. existssr ( n :: nil ). existssr (@nil nat).
+    assertsr. reflexivity. assertsr. split; auto. cbn. repeat constructor.
     reflexivity.
   - intros a b l Hl.
-    unfold halve, halve_spec, rec_fix, rec, mrec. cbn. cbn.
-    rewrite interp_mrec_bind.
-    setoid_rewrite interp_mrec_trigger. cbn.
+    unfold halve, halve_spec, rec_fix_spec, rec_spec, mrec_spec. cbn.
+    rewrite interp_mrec_spec_bind.
+    setoid_rewrite interp_mrec_spec_trigger. cbn.
     match goal with |- padded_refines_eq eq (ITree.bind ?h _) _ => set h as t end.
     assert (t = halve l).
-    { unfold halve, rec_fix, rec, t. reflexivity. }
-    rewrite H. clear H t. etransitivity.
-    eapply padded_refines_bind; eauto. intros; subst. destruct r2 as [l1 l2].
-    rewrite interp_mrec_ret. Unshelve. 3 : { apply (fun '(l1,l2) => Ret (a :: l1, b :: l2) ). } cbn. reflexivity.
+    { unfold halve, rec_fix_spec, rec_spec, t. reflexivity. }
+    rewrite H. rewrite Hl. 
     cbn. rewrite bind_bind.
     existssl. intros l1. setoid_rewrite bind_bind. existssl. intros l2.
-    existssr (a :: l1). existssr (b :: l2). rewrite bind_bind.
-    apply padded_assert_pad_eliml. intros. apply padded_assert_pad_elim.
+    rewrite bind_bind. assertsl. intros Hperm. rewrite bind_bind.
+    assertsl. intros [Hlen1 Hlen2].
+    existssr (a :: l1). existssr (b :: l2). rewrite bind_ret_l.
+    rewrite interp_mrec_spec_ret.
+    assertsr.
     { (* this is a permutation fact *) cbn. rewrite Permutation_app_comm. cbn.
-      rewrite H. rewrite Permutation_app_comm. reflexivity. }
-    rewrite bind_ret_l. reflexivity.
+      rewrite Hperm. rewrite Permutation_app_comm. reflexivity. }
+    assertsr.
+    { split; cbn. lia. apply Permutation_length in Hperm.
+      rewrite Hperm, app_length. lia. 
+    }
+    reflexivity.
 Qed.
-(*got everything except a single Permutation fact*)
+
+Lemma merge_correct' E l1 l2 : padded_refines_eq eq (merge (l1,l2)) 
+                                                    (@merge_spec' E l1 l2).
+Proof.
+  revert l2. induction l1. intro l2.
+  - cbn. unfold merge, rec_fix_spec, rec_spec, mrec_spec. cbn.
+    destruct l2; setoid_rewrite interp_mrec_spec_ret.
+    + assumesr. intro Hnil. assumesr. intros _ . existssr (@nil nat).
+      assertsr. auto. assertsr; reflexivity.
+    + assumesr. intros _ . assumesr. intros Hnl. existssr (n :: l2).
+      assertsr. auto. assertsr; reflexivity.
+  - intro l2. induction l2.
+    + setoid_rewrite interp_mrec_spec_ret. cbn.
+      assumesr. intros Hal. assumesr. intros Hnl. existssr (a :: l1).
+      assertsr. auto. assertsr; try reflexivity. rewrite app_nil_r.
+      reflexivity.
+    + rename a0 into b. 
+      unfold merge, rec_fix_spec, rec_spec, mrec_spec. cbn.
+      destruct (Nat.leb a b) eqn : Hab; setoid_rewrite interp_mrec_spec_bind;
+        setoid_rewrite interp_mrec_spec_trigger.
+      * setoid_rewrite IHl1. cbn. setoid_rewrite interp_mrec_spec_ret.
+        cbn. rewrite bind_bind. assumesr. intros Hal1.
+        assumesr. intros Hbl2. assumesl. eapply sorted_tail; eauto.
+        rewrite bind_bind. assumesl. eauto. rewrite bind_bind.
+        existssl. intros l. rewrite bind_bind. assertsl.
+        intros. rewrite bind_bind. assertsl. intros Hl12.
+        rewrite bind_ret_l. existssr (a :: l).
+        assertsr.
+        { (*fact about permutations should be able to prove fine, maybe easier to go
+            through a List Forall def of sorted*) admit. }
+        assertsr.
+        { rewrite Hl12. reflexivity. }
+        reflexivity.
+      * setoid_rewrite IHl2. setoid_rewrite interp_mrec_spec_ret.
+        cbn. rewrite bind_bind. assumesr. intros Hal1.
+        assumesr. intros Hbl2. assumesl. auto.
+        rewrite bind_bind. assumesl. eapply sorted_tail; eauto. rewrite bind_bind.
+        existssl. intros l. rewrite bind_bind. assertsl.
+        intros. rewrite bind_bind. assertsl. intros Hl12.
+        rewrite bind_ret_l. existssr (b :: l).
+        assertsr.
+        { (* similar to before*) admit. }
+        assertsr.
+        { rewrite Hl12. rewrite (Permutation_app_comm l1 (b ::l2 ) ) .
+          cbn. rewrite Permutation_app_comm. constructor. }
+        reflexivity.
+Admitted.
+
+Section strong_nat_ind.
+  Context (P : nat -> Prop) (H0 : P 0) (Hsind : (forall m, (forall n, n <= m -> P n) -> P (S m) )).
+  Theorem strong_nat_ind (n : nat) : P n .
+  Proof.
+    set (fun n => forall k, k <= n -> P k) as Q.
+    enough (Q n).
+    { unfold Q in H. apply (H n). reflexivity. }
+    induction n; unfold Q.
+    - intros. inv H. auto.
+    - unfold Q in IHn. intros k Hk. 
+      apply PeanoNat.Nat.le_succ_r in Hk. destruct Hk; subst; auto.
+  Qed.
+End strong_nat_ind.
+
+Section strong_list_ind.
+  Context (A : Type) (P : list A -> Prop) (Hnil : P nil).
+  Context (Hsind : forall a l, (forall l', length l' <= length l -> P l') -> P (a :: l) ).
+
+  Theorem strong_list_ind (l : list A) : P l.
+  Proof.
+    remember (length l) as len. generalize dependent l.
+    set (fun n =>forall l, n = length l -> P l) as Q.
+    enough (Q len); auto.
+    apply strong_nat_ind; unfold Q.
+    - intros. destruct l; try discriminate. auto.
+    - intros m Hm l Hl. destruct l; auto. apply Hsind.
+      intros. injection Hl as Hl. subst. eapply Hm; eauto.
+  Qed.
+
+End strong_list_ind.
+
+(*ok so I seem to have isolated the problem *)
+(* I should later go back to get rewrite to do this for me *)
+Lemma halve_rewrite D E (ctx : forall T, D T -> itree_spec (D +' E) T) l :
+  padded_refines_eq eq (interp_mrec_spec ctx (halve l) ) (interp_mrec_spec ctx (halve_spec l) ).
+Proof.
+  eapply refines_proper_interp_mrec_spec_eq. auto. apply halve_correct.
+Qed.
+
+Lemma merge_rewrite D E (ctx : forall T, D T -> itree_spec (D +' E) T) l1 l2 :
+  padded_refines_eq eq (interp_mrec_spec ctx (merge (l1,l2))) 
+                    (interp_mrec_spec ctx (merge_spec' l1 l2 )).
+Proof.
+  eapply refines_proper_interp_mrec_spec_eq. auto. apply merge_correct'.
+Qed.
+
+Lemma interp_mrec_spec_exists E D T (ctx : forall T, D T -> itree_spec (D +' E) T) :
+  interp_mrec_spec ctx (spec_exists T) ≈ spec_exists T.
+Proof.
+  setoid_rewrite interp_mrec_spec'_exists.
+  cbn. apply eqit_Vis. intros.  pstep. red. cbn. constructor. auto.
+Qed.
+
+Lemma interp_mrec_spec_forall E D T (ctx : forall T, D T -> itree_spec (D +' E) T) :
+  interp_mrec_spec ctx (spec_forall T) ≈ spec_forall T.
+Proof.
+  setoid_rewrite interp_mrec_spec'_forall.
+  cbn. apply eqit_Vis. intros.  pstep. red. cbn. constructor. auto.
+Qed.
+
+Lemma interp_mrec_spec_assume E D T (ctx : forall T, D T -> itree_spec (D +' E) T) :
+  interp_mrec_spec ctx (assume_spec T) ≈ assume_spec T.
+Proof.
+  Transparent assume_spec. unfold assume_spec.
+  cbn. setoid_rewrite interp_mrec_spec_bind.
+  setoid_rewrite interp_mrec_spec'_forall. rewrite bind_vis, bind_trigger.
+  apply eqit_Vis. intros. setoid_rewrite interp_mrec_spec_ret. rewrite bind_ret_l.
+  reflexivity.
+  Opaque assume_spec.
+Qed.
+
+Lemma interp_mrec_spec_assert E D T (ctx : forall T, D T -> itree_spec (D +' E) T) :
+  interp_mrec_spec ctx (assert_spec T) ≈ assert_spec T.
+Proof.
+  Transparent assert_spec. unfold assert_spec.
+  cbn. setoid_rewrite interp_mrec_spec_bind.
+  setoid_rewrite interp_mrec_spec'_exists. rewrite bind_vis, bind_trigger.
+  apply eqit_Vis. intros. setoid_rewrite interp_mrec_spec_ret. rewrite bind_ret_l.
+  reflexivity.
+  Opaque assert_spec.
+Qed.
+
+Ltac normalize_interp_mrec_spec :=
+  match goal with
+  | |- context [ITree.bind (ITree.bind ?t ?k1) ?k2 ] => setoid_rewrite bind_bind
+  | |- context [interp_mrec_spec ?ctx (ITree.bind ?t ?k) ] => setoid_rewrite interp_mrec_spec_bind
+  | |- context [interp_mrec_spec ?ctx (spec_exists ?T) ] => setoid_rewrite interp_mrec_spec_exists
+  | |- context [interp_mrec_spec ?ctx (spec_forall ?T) ] => setoid_rewrite interp_mrec_spec_forall
+  | |- context [interp_mrec_spec ?ctx (assert_spec ?T) ] => setoid_rewrite interp_mrec_spec_assert
+  | |- context [interp_mrec_spec ?ctx (assume_spec ?T) ] => setoid_rewrite interp_mrec_spec_assume
+  end.
+
+(*may also need that the results of halve give smaller lists*)
+Theorem sort_correct E l : padded_refines_eq eq (sort l) (@sort_spec E l).
+Proof.
+  (*seems like some kind of strong induction is more useful here
+    https://softwarefoundations.cis.upenn.edu/vfa-current/Merge.html#mergesort_ind
+   *)
+  revert l.
+  apply strong_list_ind.
+  - cbn. existssr (@nil nat). assertsr. reflexivity.
+    assertsr. constructor. unfold sort, rec_fix_spec, rec_spec, mrec_spec. cbn.
+    rewrite interp_mrec_spec_ret. reflexivity.
+  - intros n l Hsind. destruct l.
+    { cbn. existssr (n :: nil). assertsr. reflexivity. assertsr. constructor.
+      unfold sort, rec_fix, rec, mrec. cbn.
+      setoid_rewrite interp_mrec_spec_ret. reflexivity. }
+    remember (n :: n0 :: l) as ln. assert (Nat.leb (length ln) 1 = false).
+    { subst. reflexivity. }
+    cbn. unfold sort, rec_fix_spec, rec_spec, mrec_spec. cbn.
+    rewrite H. rewrite interp_mrec_spec_bind. rewrite halve_rewrite.
+    cbn.
+    repeat normalize_interp_mrec_spec.
+    existssl. intros l1. repeat normalize_interp_mrec_spec. existssl. 
+    intros l2. repeat normalize_interp_mrec_spec. assertsl. intros Hln.
+    assertsl. intros Hlens. setoid_rewrite interp_mrec_spec_ret.
+    rewrite bind_ret_l. cbn. setoid_rewrite interp_mrec_spec_bind.
+    assert (Hl1 : @padded_refines_eq E _ _ eq (sort l1) (sort_spec l1) ).
+    { apply Hsind. subst. clear H. destruct Hlens.
+      destruct H0; cbn in *; lia. }
+    assert (Hl2 : @padded_refines_eq E _ _ eq (sort l2) (sort_spec l2)).
+    { apply Hsind. subst. cbn in *. destruct Hlens.
+      destruct H1; lia. }
+    assert ((interp_mrec_spec
+          (calling'
+             (fun l0 : list nat =>
+              if Nat.leb (length l0) 1
+              then Ret l0
+              else
+               ITree.bind (halve l0)
+                 (fun x : list nat * list nat =>
+                  let (l3, l4) := x in
+                  ITree.bind (call_spec l3)
+                    (fun l5 : list nat =>
+                     ITree.bind (call_spec l4) (fun l6 : list nat => merge (l5, l6))))))
+          (call_spec l1)) ≈ @sort E l1).
+    { unfold sort, rec_fix_spec, rec_spec, mrec_spec. cbn.
+      setoid_rewrite interp_mrec_spec_trigger. reflexivity. }
+    rewrite H0. clear H0.
+    rewrite Hl1. cbn. rewrite bind_bind. existssl. intros l1s.
+    rewrite bind_bind.
+    assertsl. intros Hl1p. rewrite bind_bind. assertsl. intros Hl1s_sorted.
+    rewrite bind_ret_l. setoid_rewrite interp_mrec_spec_bind.
+    setoid_rewrite interp_mrec_spec_trigger. rewrite Hl2.
+    cbn. rewrite bind_bind. existssl. intros l2s. rewrite bind_bind.
+    assertsl. intros Hl2p. rewrite bind_bind. assertsl. intros Hls2_sorted.
+    rewrite bind_ret_l.
+    rewrite merge_rewrite. cbn.
+    repeat normalize_interp_mrec_spec. assumesl. auto. assumesl. auto.
+    existssl. intros lmerge. repeat normalize_interp_mrec_spec.
+    assertsl. intros Hlmerge_sorted. assertsl. intros Hlmergep.
+    setoid_rewrite interp_mrec_spec_ret. existssr lmerge.
+    assertsr. rewrite Hlmergep, Hln. 
+    setoid_rewrite Hl1p. setoid_rewrite Hl2p. reflexivity.
+    assertsr. auto. reflexivity.
+Qed.
+(*
+Lemma merge_correct1 E l1 l2 : padded_refines_eq eq (merge (l1,l2) ) (@merge_spec1 E l1 l2).
+Proof.
+  revert l2. induction l1. intro l2.
+  - cbn. unfold merge, rec_fix, rec, mrec. cbn.
+    destruct l2.
+    + setoid_rewrite interp_mrec_ret. existssr (@nil nat).
+      apply padded_assert_pad_elim. reflexivity. reflexivity.
+    + setoid_rewrite interp_mrec_ret. existssr (n :: l2) .
+      apply padded_assert_pad_elim; reflexivity.
+  - intros l2. induction l2. cbn.
+    + unfold merge, rec_fix, rec, mrec. cbn. setoid_rewrite interp_mrec_ret.
+      eexistssr. apply padded_assert_pad_elim; try reflexivity.
+      rewrite app_nil_r. reflexivity.
+    + unfold merge, rec_fix, rec, mrec. cbn. rename a0 into b.
+      destruct (Nat.leb a b) eqn : Hab.
+      * setoid_rewrite interp_mrec_bind. 
+        match goal with |- padded_refines_eq eq (ITree.bind ?h _) _ => set h as t end.
+        assert (t ≈ merge (l1, b :: l2) ).
+        { unfold merge, rec_fix, rec, mrec. unfold t. 
+          setoid_rewrite interp_mrec_trigger. simpl.
+          unfold mrec. reflexivity. }
+        rewrite H. clear H t.
+        specialize (IHl1 (b :: l2)). setoid_rewrite interp_mrec_ret.
+        etransitivity. eapply padded_refines_bind; eauto. intros. subst.
+        Unshelve. 3 : apply (fun x => Ret (a :: x) ). reflexivity.
+        cbn. rewrite bind_bind. existssl. intros l. 
+        rewrite bind_bind.
+        apply padded_assert_pad_eliml. intros Hl. rewrite bind_ret_l.
+        existssr (a :: l). apply padded_assert_pad_elim.
+        { rewrite Hl. reflexivity. } reflexivity.
+      * setoid_rewrite interp_mrec_bind.
+        match goal with |- padded_refines_eq eq (ITree.bind ?h _) _ => set h as t end.
+        assert (t ≈ merge (a :: l1, l2) ).
+        { unfold merge, rec_fix, rec, mrec. unfold t. 
+          setoid_rewrite interp_mrec_trigger. simpl.
+          unfold mrec. reflexivity. }
+        rewrite H. clear H t. setoid_rewrite interp_mrec_ret.
+        etransitivity. eapply padded_refines_bind; eauto. intros. subst.
+        Unshelve. 3 : apply (fun x => Ret (b :: x)). reflexivity.
+        cbn. rewrite bind_bind. existssl. intros l. rewrite bind_bind.
+        apply padded_assert_pad_eliml. intros. rewrite bind_ret_l.
+        existssr (b :: l). apply padded_assert_pad_elim.
+        { rewrite H. rewrite (Permutation_app_comm (a :: l1) (b :: l2) ).
+          cbn. rewrite (Permutation_app_comm l2 (a :: l1)). cbn. reflexivity. }
+        reflexivity.
+Qed.
+
+Lemma merge_correct2 E l1 l2 : padded_refines_eq eq (merge (l1,l2) ) (@merge_spec2 E l1 l2).
+Proof.
+  revert l2. induction l1. intro l2.
+  - cbn. unfold merge, rec_fix, rec, mrec. cbn. destruct l2; rewrite interp_mrec_ret.
+    + apply padded_assume_pad_elim. intros. apply padded_assume_pad_elim.
+      intros. existssr (@nil nat). apply padded_assert_pad_elim.
+      auto. reflexivity.
+    + apply padded_assume_pad_elim. intros. apply padded_assume_pad_elim.
+      intros. existssr (n :: l2). apply padded_assert_pad_elim. auto.
+      reflexivity.
+  - intros l2. induction l2.
+    + cbn. unfold merge, rec_fix, rec, mrec. cbn. rewrite interp_mrec_ret.
+      apply padded_assume_pad_elim. intros. apply padded_assume_pad_elim.
+      intros. existssr (a :: l1). apply padded_assert_pad_elim. auto. reflexivity.
+    + unfold merge, rec_fix, rec, mrec. cbn. rename a0 into b.
+      destruct (Nat.leb a b) eqn : Hab; rewrite interp_mrec_bind.
+      * match goal with |- padded_refines_eq eq (ITree.bind ?h _) _ => set h as t end.
+        assert (t ≈ merge (l1, b :: l2) ).
+        { unfold t. unfold merge, rec_fix, rec, mrec. setoid_rewrite interp_mrec_trigger.
+          cbn. unfold mrec. reflexivity. }
+        rewrite H. setoid_rewrite interp_mrec_ret.
+        etransitivity. eapply padded_refines_bind; try eapply IHl1.
+        intros. subst. Unshelve. 3 : apply (fun x => Ret (a :: x)). reflexivity.
+        cbn. rewrite bind_bind. apply padded_assume_pad_elim.
+        intros Hal1. cbn.
+        apply padded_assume_pad_elim. intros Hbl2.
+        apply padded_assume_pad_eliml. eapply sorted_tail. eauto.
+        rewrite bind_bind. apply padded_assume_pad_eliml. auto.
+        rewrite bind_bind. existssl. intros l. rewrite bind_bind.
+        apply padded_assert_pad_eliml. intros. rewrite bind_ret_l.
+        existssr (a :: l).
+        apply padded_assert_pad_elim.
+        { (* if I use mrege_spec1 I could get the assumption that l is a perm 
+             of b :: l1 ++ l2
+             then I can use Hab : a <= b to get that a is less than all elements of
+             l2 and Hal1 to get that it is less than all elements in l1
+
+             the thing is that the and_spec can slightly mess up the lemmas and
+             such, maybe they are hard to work with, need some smaller example
+           *)
+
+        apply padd
+Admitted.
+*)
